day1/answers/KVSortedListAdvanced.v
@@ -1,0 +1,246 @@
+From CRIS Require Import CRIS Atomic.
+From Stdlib Require Import Sorting.Sorted Lia.
+From answers Require Import KVSortedList.
+
+(** Optional advanced exercise.
+
+    [KVSortedList.v] used [ITree.iter] for [get] and a pure [list_put] call for
+    [put].  This file keeps the same abstract source and representation
+    relation.  The target insertion now visits one list cell per iterator
+    step.
+
+    The cursor splits the list into a processed prefix and an unprocessed
+    suffix:
+
+      (prefix, rest)
+
+    Each [inl] result moves one head element from [rest] to [prefix].
+    An [inr] result returns the completed sorted list. *)
+
+Module IterPutTarget. Section IterPutTarget.
+  Context `{!crisG Γ Σ α β τ _S _I}.
+  Import SortedListTarget.
+
+  Definition put_cursor := (entries * entries)%type.
+
+  Definition put_step (k v : Z)
+      (cursor : put_cursor) : itree crisE (put_cursor + entries) :=
+    let '(prefix, rest) := cursor in
+    match rest with
+    | [] =>
+        Ret (inr (prefix ++ [(k, v)]))
+    | (k', v') :: tl =>
+        match Z.compare k k' with
+        | Lt =>
+            Ret (inr (prefix ++ (k, v) :: rest))
+        | Eq =>
+            Ret (inr (prefix ++ (k, v) :: tl))
+        | Gt =>
+            Ret (inl (prefix ++ [(k', v')], tl))
+        end
+    end.
+
+  Definition iter_put (k v : Z) (xs : entries) : itree crisE entries :=
+    ITree.iter (put_step k v) ([], xs).
+
+  Definition scopes := [KVHdr.mn].
+  Definition v_entries := KVHdr.mn ↯ "entries".
+
+  Definition get : Z -> itree crisE (option Z) :=
+    SortedListTarget.get.
+
+  Definition put : Z * Z -> itree crisE () :=
+    fun kv =>
+      let '(k, v) := kv in
+      'xs : entries <- cgetU v_entries;;
+      ys <- iter_put k v xs;;
+      cput v_entries ys;;;
+      Ret tt.
+
+  Definition fnsems : fnsemmap :=
+    {[fid KVHdr.get #
+        (msk_scp scopes msk_true,
+          (fsp_none, cfunU KVHdr.get get));
+      fid KVHdr.put #
+        (msk_scp scopes msk_true,
+          (fsp_none, cfunU KVHdr.put put))]}.
+
+  Program Definition smod : SMod.t := {|
+    SMod.scopes := scopes;
+    SMod.fnsems := fnsems;
+    SMod.initial_st := {[v_entries # ([] : entries)↑]};
+  |}.
+  Solve All Obligations with mod_tac.
+
+  Definition t := SMod.to_mod ∅ smod.
+End IterPutTarget. End IterPutTarget.
+
+Module KVSortedListAdvancedProof.
+  Import KVSource SortedListTarget IterPutTarget.
+
+  Definition state_rel := KVSortedListProof.state_rel.
+
+  Section Refinement.
+    Context `{!crisG Γ Σ α β τ _S _I}.
+
+    Definition IstLocal : ist_type Σ :=
+      fun st_src st_tgt =>
+        (∃ m xs,
+          ⌜st_src = {[KVSource.v_map # m↑]} /\
+           st_tgt = {[IterPutTarget.v_entries # xs↑]} /\
+           state_rel m xs⌝)%I.
+
+    Local Definition Source := KVSource.t.
+    Local Definition Target := IterPutTarget.t.
+
+    Definition Ist : ist_type Σ :=
+      IstProd (IstSB Source.(Mod.scopes) IstLocal) IstEq.
+
+    Lemma Ist_from_state_rel m xs st :
+      ⌜state_rel m xs⌝ ⊢ Ist
+        (union_with uwnd {[KVSource.v_map # m↑]} st)
+        (union_with uwnd {[IterPutTarget.v_entries # xs↑]} st).
+    Proof.
+      iIntros "%Hrel".
+      unfold Ist, IstProd, IstSB, IstLocal, IstEq.
+      iExists
+        {[KVSource.v_map # m↑]},
+        {[IterPutTarget.v_entries # xs↑]}, st, st.
+      iSplit; [iPureIntro; split; ss |].
+      iSplit.
+      - iSplit; [iPureIntro; split; set_solver |].
+        iExists m, xs. iPureIntro.
+        destruct Hrel as [Hsorted Hlookup].
+        repeat split; try reflexivity; assumption.
+      - iPureIntro. reflexivity.
+    Qed.
+
+    Lemma simF_put :
+      ISim.sim_fun open Source Target Ist (fid KVHdr.put).
+    Proof.
+      cStartFunSim.
+      unfold KVSource.put, IterPutTarget.put.
+      cStepsS.
+      lazymatch goal with
+      | arg : Any.t |- _ =>
+          destruct (Any.downcast arg) as [[k v]|] eqn:Harg;
+            cStepsS; [|done]
+      end.
+      cStepsT.
+      iDestruct "IST" as
+        (st_srcL st_tgtL st_srcR st_tgtR) "%Hparts".
+      destruct Hparts as
+        [[Hsrc Htgt]
+         [[[Hscope_src Hscope_tgt]
+           [m [xs [HsrcL [HtgtL Hrel]]]]]
+          Hright]].
+      subst st_src st_tgt st_srcL st_tgtL st_srcR.
+      cStepsS. cStepsT.
+      pose proof
+        (KVSortedListProof.state_rel_put m xs k v Hrel) as Hupdated.
+      unfold IterPutTarget.iter_put.
+      assert (Hcursor :
+        [] ++ list_put k v xs = list_put k v xs) by reflexivity.
+      revert Hcursor.
+      generalize (@nil (Z * Z)) as prefix.
+      generalize xs at 1 4. iIntros (cursor prefix Hcursor).
+      iInduction cursor as [|[k' v'] tl] "IH" forall (prefix Hcursor).
+      - aUnfoldT.
+        cStepT. cStep.
+        iSplit; [eauto |].
+        iApply (Ist_from_state_rel _ _ st_tgtR).
+        iPureIntro.
+        simpl in Hcursor.
+        rewrite Hcursor.
+        exact Hupdated.
+      - aUnfoldT. unfold IterPutTarget.put_step.
+        destruct (Z.compare k k') eqn:Hcmp.
+        + cStepT. cStep.
+          iSplit; [eauto |].
+          iApply (Ist_from_state_rel _ _ st_tgtR).
+          iPureIntro.
+          simpl in Hcursor. rewrite Hcmp in Hcursor.
+          rewrite Hcursor.
+          exact Hupdated.
+        + cStepT. cStep.
+          iSplit; [eauto |].
+          iApply (Ist_from_state_rel _ _ st_tgtR).
+          iPureIntro.
+          simpl in Hcursor. rewrite Hcmp in Hcursor.
+          rewrite Hcursor.
+          exact Hupdated.
+        + cStepT.
+          iApply ("IH" $! (prefix ++ [(k', v')])).
+          iPureIntro.
+          simpl in Hcursor. rewrite Hcmp in Hcursor.
+          rewrite <- app_assoc. simpl.
+          exact Hcursor.
+    Qed.
+
+    Lemma simF_get :
+      ISim.sim_fun open Source Target Ist (fid KVHdr.get).
+    Proof.
+      cStartFunSim.
+      unfold KVSource.get, IterPutTarget.get, SortedListTarget.get.
+      cStepsS.
+      lazymatch goal with
+      | arg : Any.t |- _ =>
+          destruct (Any.downcast arg) as [k|] eqn:Harg;
+            cStepsS; [|done]
+      end.
+      cStepsT.
+      iDestruct "IST" as
+        (st_srcL st_tgtL st_srcR st_tgtR) "%Hparts".
+      destruct Hparts as
+        [[Hsrc Htgt]
+         [[[Hscope_src Hscope_tgt]
+           [m [xs [HsrcL [HtgtL Hrel]]]]]
+          Hright]].
+      subst st_src st_tgt st_srcL st_tgtL st_srcR.
+      cStepsS. cStepsT.
+      pose proof Hrel as Hstate.
+      destruct Hrel as [_ Hlookup]. rewrite Hlookup.
+      generalize xs at 1 3. iIntros (cursor).
+      iInduction cursor as [|[k' v'] tl] "IH".
+      - aUnfoldT.
+        cStep.
+        iSplit; [eauto |].
+        iApply (Ist_from_state_rel _ _ st_tgtR).
+        iPureIntro.
+        exact Hstate.
+      - aUnfoldT. simpl. destruct (Z.compare k k') eqn:Hcmp.
+        + cStep.
+          iSplit; [eauto |].
+          iApply (Ist_from_state_rel _ _ st_tgtR).
+          iPureIntro.
+          exact Hstate.
+        + cStep.
+          iSplit; [eauto |].
+          iApply (Ist_from_state_rel _ _ st_tgtR).
+          iPureIntro.
+          exact Hstate.
+        + cStepT. iApply "IH".
+    Qed.
+
+    Lemma sim : ISim.t open Source Target emp%I Ist.
+    Proof.
+      cStartModSim.
+      - unfold Source, Target, Ist. unfold_mod.
+        iIntros "_". unfold IstProd, IstSB, IstLocal, IstEq.
+        iExists {[KVSource.v_map # KVSource.empty_map↑]},
+          {[IterPutTarget.v_entries # ([] : entries)↑]}, ∅, ∅.
+        iSplit; [iPureIntro; split; ss |].
+        iSplit.
+        + iSplit; [iPureIntro; split; set_solver |].
+          iExists KVSource.empty_map, ([] : entries).
+          iPureIntro. repeat split; try reflexivity.
+          apply KVSortedListProof.state_rel_empty.
+        + iPureIntro. reflexivity.
+      - apply simF_get.
+      - apply simF_put.
+    Qed.
+
+    Lemma ctxr : ⊢ ctx_refines Target Source.
+    Proof. eapply main_adequacy, sim. Qed.
+  End Refinement.
+End KVSortedListAdvancedProof.
